boogie/sorted-list/insert.bpl
@@ -6,16 +6,16 @@
 //
 // Verification of Sorted List Insert.
 
-//SETUP:num_paths=3; (number of paths in the program)
+//SETUP:num_paths=5; (number of paths in the program)
 
 procedure SortedListInsertContract(x: Ref, k: int) returns (ret: Ref);
     requires RefSetsEqual(Br, EmptyRefSet);
-    requires LC(C.k, C.next, C.prev, C.keys, C.repr, C.sorted, C.rev_sorted, x, alloc);
+    requires LC(C.k, C.next, C.prev, C.keys, C.repr, C.sorted, C.rev_sorted, x);
     requires x != null ==> C.sorted[x];
     modifies Br, alloc, C.k, C.next, C.prev, C.keys, C.repr, C.sorted, C.rev_sorted;
     ensures RefSetSubset(old(alloc), alloc);
     ensures ret != null;
-    ensures LC(C.k, C.next, C.prev, C.keys, C.repr, C.sorted, C.rev_sorted, ret, alloc);
+    ensures LC(C.k, C.next, C.prev, C.keys, C.repr, C.sorted, C.rev_sorted, ret);
     ensures C.sorted[ret];
     ensures C.k[ret] == (if x != null && old(C.k)[x] <= k then old(C.k)[x] else k);
     ensures KeySetsEqual(C.keys[ret], (if x == null then EmptyKeySet else old(C.keys)[x])[k := true]);
@@ -31,12 +31,12 @@ procedure SortedListInsertContract(x: Ref, k: int) returns (ret: Ref);
 
 procedure SortedListInsert(x: Ref, k: int) returns (ret: Ref)
     requires RefSetsEqual(Br, EmptyRefSet);
-    requires LC(C.k, C.next, C.prev, C.keys, C.repr, C.sorted, C.rev_sorted, x, alloc);
+    requires LC(C.k, C.next, C.prev, C.keys, C.repr, C.sorted, C.rev_sorted, x);
     requires x != null ==> C.sorted[x];
     modifies Br, alloc, C.k, C.next, C.prev, C.keys, C.repr, C.sorted, C.rev_sorted;
     ensures RefSetSubset(old(alloc), alloc);
     ensures ret != null;
-    ensures LC(C.k, C.next, C.prev, C.keys, C.repr, C.sorted, C.rev_sorted, ret, alloc);
+    ensures LC(C.k, C.next, C.prev, C.keys, C.repr, C.sorted, C.rev_sorted, ret);
     ensures C.sorted[ret];
     ensures C.k[ret] == (if x != null && old(C.k)[x] <= k then old(C.k)[x] else k);
     ensures KeySetsEqual(C.keys[ret], (if x == null then EmptyKeySet else old(C.keys)[x])[k := true]);
@@ -55,6 +55,17 @@ procedure SortedListInsert(x: Ref, k: int) returns (ret: Ref)
     var tmp: Ref;
     var oldnext: Ref;
 
+    // Subexpressions
+    var node_next: Ref;
+    var node_next_keys: KeySet;
+    var node_next_repr: RefSet;
+    var node_k: int;
+    var x_next: Ref;
+    var x_next_keys: KeySet;
+    var x_next_repr: RefSet;
+    var x_k: int;
+
+    call InAllocParam(x);
     if (x == null) {
         call node := Create(k);
         call Set_keys(node, EmptyKeySet[k := true]);
@@ -69,8 +80,14 @@ procedure SortedListInsert(x: Ref, k: int) returns (ret: Ref)
         call node := Create(k);
         call Set_next(node, x);
         call Set_prev(node, null);
-        call Set_keys(node, (if C.next[node] == null then EmptyKeySet else C.keys[C.next[node]])[C.k[node] := true]);
-        call Set_repr(node, (if C.next[node] == null then EmptyRefSet else C.repr[C.next[node]])[node := true]);
+        call node_next := Get_next(node);
+        call node_k := Get_k(node);
+        if (node_next != null) {
+            call node_next_keys := Get_keys(node_next);
+            call node_next_repr := Get_repr(node_next);
+        }
+        call Set_keys(node, (if node_next == null then EmptyKeySet else node_next_keys)[node_k := true]);
+        call Set_repr(node, (if node_next == null then EmptyRefSet else node_next_repr)[node := true]);
         call Set_sorted(node, true);
         call Set_rev_sorted(node, false);
         call Set_prev(x, node);
@@ -80,20 +97,28 @@ procedure SortedListInsert(x: Ref, k: int) returns (ret: Ref)
 
         ret := node;
     } else {
-        call IfNotBr_ThenLC(C.next[x]);
+        call x_next := Get_next(x);
 
-        call tmp := SortedListInsertContract(C.next[x], k);
+        call IfNotBr_ThenLC(x_next);
+        call tmp := SortedListInsertContract(x_next, k);
 
-        call IfNotBr_ThenLC(C.next[x]);
+        call x_next := Get_next(x);
+        call IfNotBr_ThenLC(x_next);
 
-        oldnext := C.next[x];
+        oldnext := x_next;
         call Set_prev(tmp, x);
         call Set_next(x, tmp);
         call AssertLCAndRemove(tmp);
         call AssertLCAndRemove(oldnext);
 
-        call Set_keys(x, (if C.next[x] == null then EmptyKeySet else C.keys[C.next[x]])[C.k[x] := true]);
-        call Set_repr(x, (if C.next[x] == null then EmptyRefSet else C.repr[C.next[x]])[x := true]);
+        call x_next := Get_next(x);
+        call x_k := Get_k(x);
+        if (x_next != null) {
+            call x_next_keys := Get_keys(x_next);
+            call x_next_repr := Get_repr(x_next);
+        }
+        call Set_keys(x, (if x_next == null then EmptyKeySet else x_next_keys)[x_k := true]);
+        call Set_repr(x, (if x_next == null then EmptyRefSet else x_next_repr)[x := true]);
         call Set_prev(x, null);
 
         call AssertLCAndRemove(x);
